WIP

src/Experiments/FancyMachineBarrett256.v
@@ -1,3 +1,468 @@
+Require Import Coq.Classes.RelationClasses Coq.Classes.Morphisms.
+Require Import Coq.ZArith.ZArith.
+Require Import Crypto.BoundedArithmetic.Interface.
+Require Import Crypto.BoundedArithmetic.ArchitectureToZLike.
+Require Import Crypto.BoundedArithmetic.ArchitectureToZLikeProofs.
+Require Import Crypto.ModularArithmetic.BarrettReduction.ZBounded.
+Require Import Crypto.ModularArithmetic.BarrettReduction.ZHandbook.
+Require Import Crypto.Util.Tuple Crypto.Util.Option Crypto.Util.Sigma Crypto.Util.Prod.
+Require Import Crypto.Reflection.Syntax.
+Require Import Crypto.Reflection.Linearize.
+Require Import Crypto.Reflection.CommonSubexpressionElimination.
+Require Import Crypto.Reflection.Reify.
+Require Import Crypto.Util.ZUtil.
+Require Import Crypto.Util.Notations.
+
+Local Open Scope Z_scope.
+Notation eta x := (fst x, snd x).
+Notation eta3 x := (eta (fst x), snd x).
+Notation eta3' x := (fst x, eta (snd x)).
+
+Section reflection.
+  Context (ops : fancy_machine.instructions (2 * 128)).
+  Local Set Boolean Equality Schemes.
+  Local Set Decidable Equality Schemes.
+  Inductive base_type := TZ | Tbool | TW.
+  Definition interp_base_type (v : base_type) : Type :=
+    match v with
+    | TZ => Z
+    | Tbool => bool
+    | TW => fancy_machine.W
+    end.
+  Local Notation tZ := (Tbase TZ).
+  Local Notation tbool := (Tbase Tbool).
+  Local Notation tW := (Tbase TW).
+  Local Open Scope ctype_scope.
+  Inductive op : flat_type base_type -> flat_type base_type -> Type :=
+  | OPldi     : op tZ tW
+  | OPshrd    : op (tW * tW * tZ) tW
+  | OPshl     : op (tW * tZ) tW
+  | OPshr     : op (tW * tZ) tW
+  | OPmkl     : op (tW * tZ) tW
+  | OPadc     : op (tW * tW * tbool) (tbool * tW)
+  | OPsubc    : op (tW * tW * tbool) (tbool * tW)
+  | OPmulhwll : op (tW * tW) tW
+  | OPmulhwhl : op (tW * tW) tW
+  | OPmulhwhh : op (tW * tW) tW
+  | OPselc    : op (tbool * tW * tW) tW
+  | OPaddm    : op (tW * tW * tW) tW.
+
+  Definition interp_op src dst (f : op src dst)
+    : interp_flat_type_gen interp_base_type src -> interp_flat_type_gen interp_base_type dst
+    := match f in op s d return interp_flat_type_gen _ s -> interp_flat_type_gen _ d with
+       | OPldi     => ldi
+       | OPshrd    => fun xyz => let '(x, y, z) := eta3 xyz in shrd x y z
+       | OPshl     => fun xy => let '(x, y) := eta xy in shl x y
+       | OPshr     => fun xy => let '(x, y) := eta xy in shr x y
+       | OPmkl     => fun xy => let '(x, y) := eta xy in mkl x y
+       | OPadc     => fun xyz => let '(x, y, z) := eta3 xyz in adc x y z
+       | OPsubc    => fun xyz => let '(x, y, z) := eta3 xyz in subc x y z
+       | OPmulhwll => fun xy => let '(x, y) := eta xy in mulhwll x y
+       | OPmulhwhl => fun xy => let '(x, y) := eta xy in mulhwhl x y
+       | OPmulhwhh => fun xy => let '(x, y) := eta xy in mulhwhh x y
+       | OPselc    => fun xyz => let '(x, y, z) := eta3 xyz in selc x y z
+       | OPaddm    => fun xyz => let '(x, y, z) := eta3 xyz in addm x y z
+       end.
+
+  Inductive SConstT := ZConst (_ : Z) | BoolConst (_ : bool) | INVALID_CONST.
+  Inductive op_code : Set :=
+  | SOPldi | SOPshrd | SOPshl | SOPshr | SOPmkl | SOPadc | SOPsubc
+  | SOPmulhwll | SOPmulhwhl | SOPmulhwhh | SOPselc | SOPaddm.
+
+  Definition symbolicify_const (t : base_type) : interp_base_type t -> SConstT
+    := match t with
+       | TZ => fun x => ZConst x
+       | Tbool => fun x => BoolConst x
+       | TW => fun x => INVALID_CONST
+       end.
+  Definition symbolicify_op s d (v : op s d) : op_code
+    := match v with
+       | OPldi => SOPldi
+       | OPshrd => SOPshrd
+       | OPshl => SOPshl
+       | OPshr => SOPshr
+       | OPmkl => SOPmkl
+       | OPadc => SOPadc
+       | OPsubc => SOPsubc
+       | OPmulhwll => SOPmulhwll
+       | OPmulhwhl => SOPmulhwhl
+       | OPmulhwhh => SOPmulhwhh
+       | OPselc => SOPselc
+       | OPaddm => SOPaddm
+       end.
+
+  Definition CSE {t} e := @CSE base_type SConstT op_code base_type_beq SConstT_beq op_code_beq internal_base_type_dec_bl interp_base_type op symbolicify_const symbolicify_op t e (fun _ => nil).
+End reflection.
+Section instances.
+  Context {ops : fancy_machine.instructions (2 * 128)}.
+  Global Instance: forall x, reify_op op (ldi x) 1 OPldi := fun _ => I.
+  Global Instance: forall x y z, reify_op op (shrd x y z) 3 OPshrd := fun _ _ _ => I.
+  Global Instance: forall x y, reify_op op (shl x y) 2 OPshl := fun _ _ => I.
+  Global Instance: forall x y, reify_op op (shr x y) 2 OPshr := fun _ _ => I.
+  Global Instance: forall x y, reify_op op (mkl x y) 2 OPmkl := fun _ _ => I.
+  Global Instance: forall x y z, reify_op op (adc x y z) 3 OPadc := fun _ _ _ => I.
+  Global Instance: forall x y z, reify_op op (subc x y z) 3 OPsubc := fun _ _ _ => I.
+  Global Instance: forall x y, reify_op op (mulhwll x y) 2 OPmulhwll := fun _ _ => I.
+  Global Instance: forall x y, reify_op op (mulhwhl x y) 2 OPmulhwhl := fun _ _ => I.
+  Global Instance: forall x y, reify_op op (mulhwhh x y) 2 OPmulhwhh := fun _ _ => I.
+  Global Instance: forall x y z, reify_op op (selc x y z) 3 OPselc := fun _ _ _ => I.
+  Global Instance: forall x y z, reify_op op (addm x y z) 3 OPaddm := fun _ _ _ => I.
+  Global Instance: reify type Z := TZ.
+  Global Instance: reify type bool := Tbool.
+  Global Instance: reify type fancy_machine.W := TW.
+End instances.
+Ltac Reify' e := Reify.Reify' base_type (interp_base_type _) op e.
+Ltac Reify e := Reify.Reify base_type (interp_base_type _) op e.
+Ltac Reify_rhs := Reify.Reify_rhs base_type (interp_base_type _) op (interp_op _).
+
+Section syn.
+  Context {var : base_type -> Type}.
+  Inductive syntax :=
+  | RegPInv
+  | RegMod
+  | RegZero
+  | cConstZ : Z -> syntax
+  | cConstBool : bool -> syntax
+  | cLowerHalf : syntax -> syntax
+  | cUpperHalf : syntax -> syntax
+  | cLeftShifted : syntax -> Z -> syntax
+  | cRightShifted : syntax -> Z -> syntax
+  | cVar : var TW -> syntax
+  | cVarC : var Tbool -> syntax
+  | cBind : syntax -> (var TW -> syntax) -> syntax
+  | cBindCarry : syntax -> (var Tbool -> var TW -> syntax) -> syntax
+  | cMul128 : syntax -> syntax -> syntax
+  | cSelc : var Tbool -> syntax -> syntax -> syntax
+  | cAddc : var Tbool -> syntax -> syntax -> syntax
+  | cAddm : syntax -> syntax -> syntax
+  | cAdd : syntax -> syntax -> syntax
+  | cSub : syntax -> syntax -> syntax
+  | cPair : syntax -> syntax -> syntax
+  | cAbs {t} : (var t -> syntax) -> syntax
+  | cINVALID {T} (_ : T).
+End syn.
+
+Notation "'Return' x" := (cVar x) (at level 200).
+Notation "'c.Mul128' ( x , A , B ) , b" :=
+  (cBind (cMul128 A B) (fun x => b))
+    (at level 200, b at level 200, format "'c.Mul128' ( x ,  A ,  B ) , '//' b").
+Notation "'c.Add' ( x , A , B ) , b" :=
+  (cBindCarry (cAdd A B) (fun _ x => b))
+    (at level 200, b at level 200, format "'c.Add' ( x ,  A ,  B ) , '//' b").
+Notation "'c.Add' ( x , A , B ) , b" :=
+  (cBindCarry (cAdd (cVar A) B) (fun _ x => b))
+    (at level 200, b at level 200, format "'c.Add' ( x ,  A ,  B ) , '//' b").
+Notation "'c.Add' ( x , A , B ) , 'c.Addc' ( x1 , A1 , B1 ) , b" :=
+  (cBindCarry (cAdd A B) (fun c x => cBindCarry (cAddc c A1 B1) (fun _ x1 => b)))
+    (at level 200, b at level 200, format "'c.Add' ( x ,  A ,  B ) , '//' 'c.Addc' ( x1 ,  A1 ,  B1 ) , '//' b").
+Notation "'c.Add' ( x , A , B ) , 'c.Addc' ( x1 , A1 , B1 ) , b" :=
+  (cBindCarry (cAdd A B) (fun c x => cBindCarry (cAddc c (cVar A1) B1) (fun _ x1 => b)))
+    (at level 200, b at level 200, format "'c.Add' ( x ,  A ,  B ) , '//' 'c.Addc' ( x1 ,  A1 ,  B1 ) , '//' b").
+Notation "'c.Add' ( x , A , B ) , 'c.Addc' ( x1 , A1 , B1 ) , b" :=
+  (cBindCarry (cAdd (cVar A) B) (fun c x => cBindCarry (cAddc c A1 B1) (fun _ x1 => b)))
+    (at level 200, b at level 200, format "'c.Add' ( x ,  A ,  B ) , '//' 'c.Addc' ( x1 ,  A1 ,  B1 ) , '//' b").
+Notation "'c.Add' ( x , A , B ) , 'c.Addc' ( x1 , A1 , B1 ) , b" :=
+  (cBindCarry (cAdd (cVar A) B) (fun c x => cBindCarry (cAddc c (cVar A1) B1) (fun _ x1 => b)))
+    (at level 200, b at level 200, format "'c.Add' ( x ,  A ,  B ) , '//' 'c.Addc' ( x1 ,  A1 ,  B1 ) , '//' b").
+Notation "'c.Add' ( x , A , B ) , 'c.Addc' ( x1 , A1 , B1 ) , 'c.Selc' ( x2 , A2 , B2 ) , b" :=
+  (cBindCarry (cAdd A B) (fun c x => cBindCarry (cAddc c A1 B1) (fun c1 x1 => cBind (cSelc c1 A2 B2) (fun x2 => b))))
+    (at level 200, b at level 200, format "'c.Add' ( x ,  A ,  B ) , '//' 'c.Addc' ( x1 ,  A1 ,  B1 ) , '//' 'c.Selc' ( x2 ,  A2 ,  B2 ) , '//' b").
+Notation "'c.Add' ( x , A , B ) , 'c.Addc' ( x1 , A1 , B1 ) , 'c.Selc' ( x2 , A2 , B2 ) , b" :=
+  (cBindCarry (cAdd (cVar A) B) (fun c x => cBindCarry (cAddc c A1 B1) (fun c1 x1 => cBind (cSelc c1 A2 B2) (fun x2 => b))))
+    (at level 200, b at level 200, format "'c.Add' ( x ,  A ,  B ) , '//' 'c.Addc' ( x1 ,  A1 ,  B1 ) , '//' 'c.Selc' ( x2 ,  A2 ,  B2 ) , '//' b").
+Notation "'c.Add' ( x , A , B ) , 'c.Addc' ( x1 , A1 , B1 ) , 'c.Selc' ( x2 , A2 , B2 ) , b" :=
+  (cBindCarry (cAdd A B) (fun c x => cBindCarry (cAddc c (cVar A1) B1) (fun c1 x1 => cBind (cSelc c1 A2 B2) (fun x2 => b))))
+    (at level 200, b at level 200, format "'c.Add' ( x ,  A ,  B ) , '//' 'c.Addc' ( x1 ,  A1 ,  B1 ) , '//' 'c.Selc' ( x2 ,  A2 ,  B2 ) , '//' b").
+Notation "'c.Add' ( x , A , B ) , 'c.Addc' ( x1 , A1 , B1 ) , 'c.Selc' ( x2 , A2 , B2 ) , b" :=
+  (cBindCarry (cAdd (cVar A) B) (fun c x => cBindCarry (cAddc c (cVar A1) B1) (fun c1 x1 => cBind (cSelc c1 A2 B2) (fun x2 => b))))
+    (at level 200, b at level 200, format "'c.Add' ( x ,  A ,  B ) , '//' 'c.Addc' ( x1 ,  A1 ,  B1 ) , '//' 'c.Selc' ( x2 ,  A2 ,  B2 ) , '//' b").
+Notation "'c.Add' ( x , A , B ) , 'c.Addc' ( x1 , A1 , B1 ) , 'c.Selc' ( x2 , A2 , B2 ) , b" :=
+  (cBindCarry (cAdd (cVar A) (cVar B)) (fun c x => cBindCarry (cAddc c (cVar A1) (cVar B1)) (fun c1 x1 => cBind (cSelc c1 A2 B2) (fun x2 => b))))
+    (at level 200, b at level 200, format "'c.Add' ( x ,  A ,  B ) , '//' 'c.Addc' ( x1 ,  A1 ,  B1 ) , '//' 'c.Selc' ( x2 ,  A2 ,  B2 ) , '//' b").
+
+Notation "'c.Sub' ( x , A , B ) , b" :=
+  (cBindCarry (cSub A B) (fun _ x => b))
+    (at level 200, b at level 200, format "'c.Sub' ( x ,  A ,  B ) , '//' b").
+Notation "'c.Sub' ( x , A , B ) , b" :=
+  (cBindCarry (cSub (cVar A) B) (fun _ x => b))
+    (at level 200, b at level 200, format "'c.Sub' ( x ,  A ,  B ) , '//' b").
+Notation "'c.Sub' ( x , A , B ) , b" :=
+  (cBindCarry (cSub A (cVar B)) (fun _ x => b))
+    (at level 200, b at level 200, format "'c.Sub' ( x ,  A ,  B ) , '//' b").
+Notation "'c.Sub' ( x , A , B ) , b" :=
+  (cBindCarry (cSub (cVar A) (cVar B)) (fun _ x => b))
+    (at level 200, b at level 200, format "'c.Sub' ( x ,  A ,  B ) , '//' b").
+
+Notation "'c.Addm' ( x , A , B ) , b" :=
+  (cBind (cAddm A B) (fun x => b))
+    (at level 200, b at level 200, format "'c.Addm' ( x ,  A ,  B ) , '//' b").
+Notation "'c.Addm' ( x , A , B ) , b" :=
+  (cBind (cAddm A (cVar B)) (fun x => b))
+    (at level 200, b at level 200, format "'c.Addm' ( x ,  A ,  B ) , '//' b").
+Notation "'c.Addm' ( x , A , B ) , b" :=
+  (cBind (cAddm (cVar A) B) (fun x => b))
+    (at level 200, b at level 200, format "'c.Addm' ( x ,  A ,  B ) , '//' b").
+Notation "'c.Addm' ( x , A , B ) , b" :=
+  (cBind (cAddm (cVar A) (cVar B)) (fun x => b))
+    (at level 200, b at level 200, format "'c.Addm' ( x ,  A ,  B ) , '//' b").
+
+Notation "'c.LowerHalf' ( x )" :=
+  (cLowerHalf x)
+    (at level 200, format "'c.LowerHalf' ( x )").
+Notation "'c.LowerHalf' ( x )" :=
+  (cLowerHalf (cVar x))
+    (at level 200, format "'c.LowerHalf' ( x )").
+Notation "'c.UpperHalf' ( x )" :=
+  (cUpperHalf x)
+    (at level 200, format "'c.UpperHalf' ( x )").
+Notation "'c.UpperHalf' ( x )" :=
+  (cUpperHalf (cVar x))
+    (at level 200, format "'c.UpperHalf' ( x )").
+Notation "'c.LeftShifted' { x , v }" :=
+  (cLeftShifted x v)
+    (at level 200, format "'c.LeftShifted' { x ,  v }").
+Notation "'c.LeftShifted' { x , v }" :=
+  (cLeftShifted (cVar x) v)
+    (at level 200, format "'c.LeftShifted' { x ,  v }").
+Notation "'c.RightShifted' { x , v }" :=
+  (cRightShifted x v)
+    (at level 200, format "'c.RightShifted' { x ,  v }").
+Notation "'c.RightShifted' { x , v }" :=
+  (cRightShifted (cVar x) v)
+    (at level 200, format "'c.RightShifted' { x ,  v }").
+Notation "'λ'  x .. y , t" := (cAbs (fun x => .. (cAbs (fun y => t)) ..))
+  (at level 200, x binder, y binder, right associativity).
+
+Definition Syntax := forall var, @syntax var.
+
+Section assemble.
+  Context (ops : fancy_machine.instructions (2 * 128)).
+
+  Section with_var.
+    Context {var : base_type -> Type}.
+
+    Fixpoint assemble_syntax_const
+             {t}
+      : interp_flat_type_gen (interp_base_type _) t -> @syntax var
+      := match t return interp_flat_type_gen (interp_base_type _) t -> @syntax var with
+         | Tbase TZ => cConstZ
+         | Tbase Tbool => cConstBool
+         | Tbase t => fun _ => cINVALID t
+         | Prod A B => fun xy => cPair (@assemble_syntax_const A (fst xy))
+                                       (@assemble_syntax_const B (snd xy))
+         end.
+
+    Definition assemble_syntaxf_step
+               (assemble_syntaxf : forall {t} (v : @Syntax.exprf base_type (interp_base_type _) op (fun _ => @syntax var) t), @syntax var)
+               {t} (v : @Syntax.exprf base_type (interp_base_type _) op (fun _ => @syntax var) t) : @syntax var.
+    Proof.
+      refine match v return @syntax var with
+             | Syntax.Const t x => assemble_syntax_const x
+             | Syntax.Var _ x => x
+             | Syntax.Op t1 tR op args
+               => let v := @assemble_syntaxf t1 args in
+                  match op, v with
+                  | OPldi    , cConstZ 0 => RegZero
+                  | OPldi    , cConstZ v => cINVALID v
+                  | OPldi    , RegZero => RegZero
+                  | OPldi    , RegMod => RegMod
+                  | OPldi    , RegPInv => RegPInv
+                  | OPshrd   , _ => cINVALID op
+                  | OPshl    , cPair w (cConstZ n) => cLeftShifted w n
+                  | OPshr    , cPair w (cConstZ n) => cRightShifted w n
+                  | OPmkl    , _ => cINVALID op
+                  | OPadc    , cPair (cPair x y) (cVarC c) => cAddc c x y
+                  | OPadc    , cPair x (cPair y (cVarC c)) => cAddc c x y
+                  | OPadc    , cPair (cPair x y) (cConstBool false) => cAdd x y
+                  | OPadc    , cPair x (cPair y (cConstBool false)) => cAdd x y
+                  | OPsubc   , cPair (cPair x y) (cConstBool false) => cSub x y
+                  | OPsubc   , cPair x (cPair y (cConstBool false)) => cSub x y
+                  | OPmulhwll, cPair x y => cMul128 (cLowerHalf x) (cLowerHalf y)
+                  | OPmulhwhl, cPair x y => cMul128 (cUpperHalf x) (cLowerHalf y)
+                  | OPmulhwhh, cPair x y => cMul128 (cUpperHalf x) (cUpperHalf y)
+                  | OPselc   , cPair (cVarC c) (cPair x y) => cSelc c x y
+                  | OPselc   , cPair (cPair (cVarC c) x) y => cSelc c x y
+                  | OPaddm   , cPair x (cPair y RegMod) => cAddm x y
+                  | OPaddm   , cPair (cPair x y) RegMod => cAddm x y
+                  | _, _ => cINVALID op
+                  end
+             | Syntax.Let tx ex _ eC
+               => let ex' := @assemble_syntaxf _ ex in
+                 let eC' := fun x => @assemble_syntaxf _ (eC x) in
+                 let special := match ex' with
+                                | RegZero as ex'' | RegMod as ex'' | RegPInv as ex''
+                                | cUpperHalf _ as ex'' | cLowerHalf _ as ex''
+                                | cLeftShifted _ _ as ex''
+                                | cRightShifted _ _ as ex''
+                                  => Some ex''
+                                | _ => None
+                                end in
+                 match special, tx return (interp_flat_type_gen _ tx -> _) -> _ with
+                 | Some x, Tbase _ => fun eC' => eC' x
+                 | _, Tbase TW
+                   => fun eC' => cBind ex' (fun x => eC' (cVar x))
+                 | _, Prod (Tbase Tbool) (Tbase TW)
+                   => fun eC' => cBindCarry ex' (fun c x => eC' (cVarC c, cVar x))
+                 | _, _
+                   => fun _ => cINVALID (fun x : Prop => x)
+                 end eC'
+             | Syntax.Pair _ ex _ ey
+               => cPair (@assemble_syntaxf _ ex) (@assemble_syntaxf _ ey)
+             end.
+    Defined.
+
+    Fixpoint assemble_syntaxf {t} v {struct v} : @syntax var
+      := @assemble_syntaxf_step (@assemble_syntaxf) t v.
+    Fixpoint assemble_syntax {t} (v : @Syntax.expr base_type (interp_base_type _) op (fun _ => @syntax var) t) (args : list (@syntax var)) {struct v}
+      : @syntax var
+      := match v, args return @syntax var with
+         | Syntax.Return _ x, _ => assemble_syntaxf x
+         | Syntax.Abs _ _ f, nil => cAbs (fun x => @assemble_syntax _ (f (cVar x)) args)
+         | Syntax.Abs _ _ f, cons v vs => @assemble_syntax _ (f v) vs
+         end.
+  End with_var.
+
+  Definition AssembleSyntax {t} (v : Syntax.Expr _ _ _ t) (args : list Syntax) : Syntax
+    := fun var => @assemble_syntax var t (v _) (List.map (fun f => f var) args).
+End assemble.
+
+Section expression.
+  Let b : Z := 2.
+  Let k : Z := 253.
+  Let offset : Z := 3.
+  Context (ops : fancy_machine.instructions (2 * 128)) (props : fancy_machine.arithmetic ops).
+  (** 25519 dsa *)
+  Context (m μ : Z)
+          (m_pos : 0 < m).
+  Let base_pos : 0 < b. reflexivity. Qed.
+  Context (k_good : m < b^k)
+          (μ_good : μ = b^(2*k) / m) (* [/] is [Z.div], which is truncated *).
+  Let offset_nonneg : 0 <= offset. unfold offset; omega. Qed.
+  Let k_big_enough : offset <= k. unfold offset, k; omega. Qed.
+  Context (m_small : 3 * m <= b^(k+offset))
+          (m_large : b^(k-offset) <= m + 1).
+  Context (H : 0 <= m < 2^256).
+  Let H' : 0 <= 250 <= 256. omega. Qed.
+  Let H'' : 0 < 250. omega. Qed.
+  Let props' := ZLikeProperties_of_ArchitectureBoundedOps ops m H 250 H' H''.
+  Let ops' := (ZLikeOps_of_ArchitectureBoundedOps ops m 250).
+  Local Existing Instances props' ops'.
+  Local Notation fst' := (@fst fancy_machine.W fancy_machine.W).
+  Local Notation snd' := (@snd fancy_machine.W fancy_machine.W).
+  Local Notation SmallT := (@ZBounded.SmallT (2 ^ 256) (2 ^ 250) m
+                                  (@ZLikeOps_of_ArchitectureBoundedOps 128 ops m _)).
+  Definition ldi' : load_immediate SmallT := _.
+  Let isldi : is_load_immediate ldi' := _.
+  Axiom (μ_range : 0 <= b ^ (2 * k) / m < b ^ (k + offset)).
+  Definition μ' : SmallT := ldi' μ.
+  Let μ'_eq : ZBounded.decode_small μ' = μ.
+  Proof.
+    unfold ZBounded.decode_small, ZLikeOps_of_ArchitectureBoundedOps, μ'.
+    apply (decode_load_immediate _ _).
+    rewrite μ_good; apply μ_range.
+  Qed.
+
+  Definition pre_f v
+    := (@barrett_reduce m b k μ offset m_pos base_pos μ_good offset_nonneg k_big_enough m_small m_large ops' props' μ' I μ'_eq (fst' v, snd' v)).
+
+  Local Arguments μ' / .
+  Local Arguments ldi' / .
+
+  Definition expression'
+    := Eval simpl in
+        (fun v => proj1_sig (pre_f v)).
+  Definition expression
+    := Eval cbv beta iota delta [expression' fst snd] in
+        fun v => let RegMod := fancy_machine.ldi m in
+              let RegMu := fancy_machine.ldi μ in
+              let RegZero := fancy_machine.ldi 0 in
+              expression' v.
+
+  Definition expression_eq v H : fancy_machine.decode (expression v) = _
+    := proj1 (proj2_sig (pre_f v) H).
+End expression.
+
+Print expression.
+
+Section reflected.
+  Context (ops : fancy_machine.instructions (2 * 128)).
+  Definition rexpression : Syntax.Expr base_type (interp_base_type _) op (Arrow TZ (Arrow TZ (Arrow TW (Arrow TW (Tbase TW))))).
+  Proof.
+    let v := (eval cbv beta delta [expression] in (fun m μ x y => expression ops m μ (x, y))) in
+    let v := Reify v in
+    exact v.
+  Defined.
+
+  Definition rexpression_simple := Eval vm_compute in CSE ops (InlineConst (Linearize rexpression)).
+
+  Context (m μ : Z)
+          (props : fancy_machine.arithmetic ops).
+
+  Let result (v : tuple fancy_machine.W 2) := Syntax.Interp (interp_op _) rexpression_simple m μ (fst v) (snd v).
+
+  Theorem sanity : result = expression ops m μ.
+  Proof.
+    reflexivity.
+  Qed.
+
+  Local Infix "≡₂₅₆" := (Z.equiv_modulo (2^256)).
+  Local Infix "≡" := (Z.equiv_modulo m).
+  About expression_eq.
+  Theorem correctness
+          (b : Z := 2)
+          (k : Z := 253)
+          (offset : Z := 3)
+          (H0 : 0 < m)
+          (H1 : μ = b^(2 * k) / m)
+          (H2 : 3 * m <= b^(k + offset))
+          (H3 : b^(k - offset) <= m + 1)
+          (H4 : 0 <= m < 2^(k + offset))
+          (v : tuple fancy_machine.W 2)
+    : fancy_machine.decode (result v) = decode v mod m.
+  Proof.
+    replace m' with (fancy_machine.decode (fancy_machine.ldi m')) in H4
+      by (apply decode_load_immediate; trivial; exact _).
+    assert (H' : fancy_machine.decode (result v) ≡ decode v * R'
+                 /\ 0 <= fancy_machine.decode (result v) < modulus).
+    { rewrite sanity; destruct v; apply expression_correct; assumption. }
+    destruct H' as [H'0 H'1].
+    rewrite <- H'0.
+    rewrite Z.mod_small by assumption.
+    reflexivity.
+  Qed.
+End reflected.
+
+Definition compiled_syntax
+  := Eval vm_compute in
+      (fun ops => AssembleSyntax ops (rexpression_simple _) (@RegMod :: @RegPInv :: nil)%list).
+
+Print compiled_syntax.
+(* compiled_syntax =
+fun (_ : fancy_machine.instructions (2 * 128)) (var : base_type -> Type) =>
+λ x x0 : var TW,
+c.Mul128(x1, c.LowerHalf(x), c.LowerHalf(RegPInv)),
+c.Mul128(x2, c.UpperHalf(x), c.LowerHalf(RegPInv)),
+c.Add(x4, x1, c.LeftShifted{x2, 128}),
+c.Mul128(x5, c.UpperHalf(RegPInv), c.LowerHalf(x)),
+c.Add(x7, x4, c.LeftShifted{x5, 128}),
+c.Mul128(x8, c.UpperHalf(x7), c.UpperHalf(RegMod)),
+c.Mul128(x9, c.UpperHalf(x7), c.LowerHalf(RegMod)),
+c.Mul128(x10, c.LowerHalf(x7), c.LowerHalf(RegMod)),
+c.Add(x12, x10, c.LeftShifted{x9, 128}),
+c.Addc(x14, x8, c.RightShifted{x9, 128}),
+c.Mul128(x15, c.UpperHalf(RegMod), c.LowerHalf(x7)),
+c.Add(x17, x12, c.LeftShifted{x15, 128}),
+c.Addc(x19, x14, c.RightShifted{x15, 128}),
+c.Add(_, x, x17),
+c.Addc(x23, x0, x19),
+c.Selc(x24, RegMod, RegZero),
+c.Sub(x26, x23, x24),
+c.Addm(x27, x26, RegZero),
+Return x27
+     : fancy_machine.instructions (2 * 128) -> forall var : base_type -> Type, syntax
+*)
+
+
 Require Import Coq.Classes.RelationClasses Coq.Classes.Morphisms Coq.micromega.Psatz.
 Require Import Coq.ZArith.ZArith.
 Require Import Crypto.BoundedArithmetic.Interface.
