src/Experiments/FancyMachineMontgomery256.v
@@ -10,56 +10,13 @@ Require Import Crypto.Reflection.Syntax.
 Require Import Crypto.Reflection.Linearize.
 Require Import Crypto.Reflection.CommonSubexpressionElimination.
 Require Import Crypto.Reflection.Reify.
+Require Import Crypto.Util.ZUtil.
+Require Import Crypto.Util.Notations.
 
 Local Open Scope Z_scope.
 Notation eta x := (fst x, snd x).
 Notation eta3 x := (eta (fst x), snd x).
 Notation eta3' x := (fst x, eta (snd x)).
-
-Section expression.
-  Context (ops : fancy_machine.instructions (2 * 128)) (props : fancy_machine.arithmetic ops) (modulus : Z) (m' : Z) (Hm : modulus <> 0) (H : 0 <= modulus < 2^256) (Hm' : 0 <= m' < 2^256).
-  Let H' : 0 <= 256 <= 256. omega. Qed.
-  Let H'' : 0 < 256. omega. Qed.
-  Let props' := ZLikeProperties_of_ArchitectureBoundedOps ops modulus H 256 H' H''.
-  Let ops' := (ZLikeOps_of_ArchitectureBoundedOps ops modulus 256).
-  Local Notation fst' := (@fst fancy_machine.W fancy_machine.W).
-  Local Notation snd' := (@snd fancy_machine.W fancy_machine.W).
-  Definition ldi' : load_immediate
-                     (@ZBounded.SmallT (2 ^ 256) (2 ^ 256) modulus
-                                       (@ZLikeOps_of_ArchitectureBoundedOps 128 ops modulus 256)) := _.
-  Let isldi : is_load_immediate ldi' := _.
-  Definition pre_f := (fun v => (reduce_via_partial (2^256) modulus (props := props') (ldi' m') I Hm (fst' v, snd' v))).
-  Definition f := (fun v => proj1_sig (pre_f v)).
-
-  Local Arguments proj1_sig _ _ !_ / .
-  Local Arguments ZBounded.CarryAdd / .
-  Local Arguments ZBounded.ConditionalSubtract / .
-  Local Arguments ZBounded.ConditionalSubtractModulus / .
-  Local Arguments ZLikeOps_of_ArchitectureBoundedOps / .
-  Local Arguments ZBounded.DivBy_SmallBound / .
-  Local Arguments f / .
-  Local Arguments pre_f / .
-  Local Arguments ldi' / .
-  Local Arguments reduce_via_partial / .
-
-  Definition expression'
-    := Eval simpl in f.
-  Definition expression
-    := Eval cbv beta delta [expression' fst snd] in
-        fun v => let RegMod := fancy_machine.ldi modulus in
-                 let RegPInv := fancy_machine.ldi m' in
-                 let RegZero := fancy_machine.ldi 0 in
-                 expression' v.
-  Definition expression_eq v : fancy_machine.decode (expression v) = _
-    := proj1 (proj2_sig (pre_f v) I).
-  Definition expression_correct
-             R' HR0 HR1
-             v
-             Hv
-    : ZUtil.Z.equiv_modulo _ (fancy_machine.decode (expression v)) _
-      /\ 0 <= fancy_machine.decode (expression v) < _
-    := @ZBounded.reduce_via_partial_correct (2^256) modulus _ props' (ldi' m') I Hm R' HR0 HR1 v I Hv.
-End expression.
 
 Section reflection.
   Context (ops : fancy_machine.instructions (2 * 128)).
@@ -157,18 +114,6 @@ End instances.
 Ltac Reify' e := Reify.Reify' base_type (interp_base_type _) op e.
 Ltac Reify e := Reify.Reify base_type (interp_base_type _) op e.
 Ltac Reify_rhs := Reify.Reify_rhs base_type (interp_base_type _) op (interp_op _).
-
-Section reflected.
-  Context (ops : fancy_machine.instructions (2 * 128)).
-  Definition rexpression : Syntax.Expr base_type (interp_base_type _) op (Arrow TZ (Arrow TZ (Arrow TW (Arrow TW (Tbase TW))))).
-  Proof.
-    let v := (eval cbv beta delta [expression] in (fun modulus m' x y => expression ops modulus m' (x, y))) in
-    let v := Reify v in
-    exact v.
-  Defined.
-
-  Definition rexpression_simple := Eval vm_compute in CSE ops (InlineConst (Linearize rexpression)).
-End reflected.
 
 Section syn.
   Context {var : base_type -> Type}.
@@ -380,6 +325,98 @@ Section assemble.
   Definition AssembleSyntax {t} (v : Syntax.Expr _ _ _ t) (args : list Syntax) : Syntax
     := fun var => @assemble_syntax var t (v _) (List.map (fun f => f var) args).
 End assemble.
+
+Section expression.
+  Context (ops : fancy_machine.instructions (2 * 128)) (props : fancy_machine.arithmetic ops) (modulus : Z) (m' : Z) (Hm : modulus <> 0) (H : 0 <= modulus < 2^256) (Hm' : 0 <= m' < 2^256).
+  Let H' : 0 <= 256 <= 256. omega. Qed.
+  Let H'' : 0 < 256. omega. Qed.
+  Let props' := ZLikeProperties_of_ArchitectureBoundedOps ops modulus H 256 H' H''.
+  Let ops' := (ZLikeOps_of_ArchitectureBoundedOps ops modulus 256).
+  Local Notation fst' := (@fst fancy_machine.W fancy_machine.W).
+  Local Notation snd' := (@snd fancy_machine.W fancy_machine.W).
+  Definition ldi' : load_immediate
+                     (@ZBounded.SmallT (2 ^ 256) (2 ^ 256) modulus
+                                       (@ZLikeOps_of_ArchitectureBoundedOps 128 ops modulus 256)) := _.
+  Let isldi : is_load_immediate ldi' := _.
+  Definition pre_f := (fun v => (reduce_via_partial (2^256) modulus (props := props') (ldi' m') I Hm (fst' v, snd' v))).
+  Definition f := (fun v => proj1_sig (pre_f v)).
+
+  Local Arguments proj1_sig _ _ !_ / .
+  Local Arguments ZBounded.CarryAdd / .
+  Local Arguments ZBounded.ConditionalSubtract / .
+  Local Arguments ZBounded.ConditionalSubtractModulus / .
+  Local Arguments ZLikeOps_of_ArchitectureBoundedOps / .
+  Local Arguments ZBounded.DivBy_SmallBound / .
+  Local Arguments f / .
+  Local Arguments pre_f / .
+  Local Arguments ldi' / .
+  Local Arguments reduce_via_partial / .
+
+  Definition expression'
+    := Eval simpl in f.
+  Definition expression
+    := Eval cbv beta delta [expression' fst snd] in
+        fun v => let RegMod := fancy_machine.ldi modulus in
+                 let RegPInv := fancy_machine.ldi m' in
+                 let RegZero := fancy_machine.ldi 0 in
+                 expression' v.
+  Definition expression_eq v : fancy_machine.decode (expression v) = _
+    := proj1 (proj2_sig (pre_f v) I).
+  Definition expression_correct
+             R' HR0 HR1
+             v
+             Hv
+    : ZUtil.Z.equiv_modulo _ (fancy_machine.decode (expression v)) _
+      /\ 0 <= fancy_machine.decode (expression v) < _
+    := @ZBounded.reduce_via_partial_correct (2^256) modulus _ props' (ldi' m') I Hm R' HR0 HR1 v I Hv.
+End expression.
+
+Section reflected.
+  Context (ops : fancy_machine.instructions (2 * 128)).
+  Definition rexpression : Syntax.Expr base_type (interp_base_type _) op (Arrow TZ (Arrow TZ (Arrow TW (Arrow TW (Tbase TW))))).
+  Proof.
+    let v := (eval cbv beta delta [expression] in (fun modulus m' x y => expression ops modulus m' (x, y))) in
+    let v := Reify v in
+    exact v.
+  Defined.
+
+  Definition rexpression_simple := Eval vm_compute in CSE ops (InlineConst (Linearize rexpression)).
+
+  Context (modulus m' : Z)
+          (props : fancy_machine.arithmetic ops).
+
+  Let result (v : tuple fancy_machine.W 2) := Syntax.Interp (interp_op _) rexpression_simple modulus m' (fst v) (snd v).
+
+  Theorem sanity : result = expression ops modulus m'.
+  Proof.
+    reflexivity.
+  Qed.
+
+  Local Infix "≡₂₅₆" := (Z.equiv_modulo (2^256)).
+  Local Infix "≡" := (Z.equiv_modulo modulus).
+
+  Theorem correctness
+          R' (* modular inverse of 2^256 *)
+          (H0 : modulus <> 0)
+          (H1 : 0 <= modulus < 2^256)
+          (H2 : 0 <= m' < 2^256)
+          (H3 : 2^256 * R' ≡ 1)
+          (H4 : modulus * m' ≡₂₅₆ -1)
+          (v : tuple fancy_machine.W 2)
+          (H5 : 0 <= decode v <= 2^256 * modulus)
+    : fancy_machine.decode (result v) = (decode v * R') mod modulus.
+  Proof.
+    replace m' with (fancy_machine.decode (fancy_machine.ldi m')) in H4
+      by (apply decode_load_immediate; trivial; exact _).
+    assert (H' : fancy_machine.decode (result v) ≡ decode v * R'
+                 /\ 0 <= fancy_machine.decode (result v) < modulus).
+    { rewrite sanity; destruct v; apply expression_correct; assumption. }
+    destruct H' as [H'0 H'1].
+    rewrite <- H'0.
+    rewrite Z.mod_small by assumption.
+    reflexivity.
+  Qed.
+End reflected.
 
 Definition compiled_syntax
   := Eval vm_compute in
